concurrency/hack-hash-table/Main.s.dfy
@@ -3,6 +3,7 @@ include "HTResource.i.dfy"
 abstract module Main {
   import ARS = HTResource
   import Ifc = MapIfc
+  import opened NativeTypes
 
   type Variables(==,!new) // using this name so the impl is more readable
   predicate Inv(v: Variables)
@@ -13,8 +14,9 @@ abstract module Main {
   ensures Inv(v)
 
   method call(v: Variables, input: Ifc.Input,
-      rid: int, glinear in_r: ARS.R, thread_id: nat)
+      rid: int, glinear in_r: ARS.R, thread_id: uint32)
   returns (output: Ifc.Output, glinear out_r: ARS.R)
+  decreases * // boi I don't feel bad about this
   requires Inv(v)
   requires in_r == ARS.input_ticket(rid, input)
   ensures out_r == ARS.output_stub(rid, output)
